execspec: checking in current generated files (not final)

spec/design/ARM_HYP/ArchStructures_H.thy
@@ -14,7 +14,7 @@ imports
   "../Types_H"
   Hardware_H
 begin
-context Arch begin global_naming ARM_H
+context Arch begin global_naming ARM_HYP_H
 
 type_synonym asid = "word32"
 
@@ -29,6 +29,12 @@ datatype arch_capability =
   | PageCap machine_word vmrights vmpage_size "(asid * vptr) option"
   | PageTableCap machine_word "(asid * vptr) option"
   | PageDirectoryCap machine_word "asid option"
+  | VCPUCap machine_word
+
+primrec
+  capVCPUPtr :: "arch_capability \<Rightarrow> machine_word"
+where
+  "capVCPUPtr (VCPUCap v0) = v0"
 
 primrec
   capVPBasePtr :: "arch_capability \<Rightarrow> machine_word"
@@ -79,6 +85,11 @@ primrec
   capVPMappedAddress :: "arch_capability \<Rightarrow> (asid * vptr) option"
 where
   "capVPMappedAddress (PageCap v0 v1 v2 v3) = v3"
+
+primrec
+  capVCPUPtr_update :: "(machine_word \<Rightarrow> machine_word) \<Rightarrow> arch_capability \<Rightarrow> arch_capability"
+where
+  "capVCPUPtr_update f (VCPUCap v0) = VCPUCap (f v0)"
 
 primrec
   capVPBasePtr_update :: "(machine_word \<Rightarrow> machine_word) \<Rightarrow> arch_capability \<Rightarrow> arch_capability"
@@ -150,6 +161,11 @@ abbreviation (input)
 where
   "PageDirectoryCap_ \<lparr> capPDBasePtr= v0, capPDMappedASID= v1 \<rparr> == PageDirectoryCap v0 v1"
 
+abbreviation (input)
+  VCPUCap_trans :: "(machine_word) \<Rightarrow> arch_capability" ("VCPUCap'_ \<lparr> capVCPUPtr= _ \<rparr>")
+where
+  "VCPUCap_ \<lparr> capVCPUPtr= v0 \<rparr> == VCPUCap v0"
+
 definition
   isASIDPoolCap :: "arch_capability \<Rightarrow> bool"
 where
@@ -185,13 +201,139 @@ where
     PageDirectoryCap v0 v1 \<Rightarrow> True
   | _ \<Rightarrow> False"
 
+definition
+  isVCPUCap :: "arch_capability \<Rightarrow> bool"
+where
+ "isVCPUCap v \<equiv> case v of
+    VCPUCap v0 \<Rightarrow> True
+  | _ \<Rightarrow> False"
+
 datatype asidpool =
     ASIDPool "asid \<Rightarrow> ((machine_word) option)"
+
+datatype vcpu =
+    VCPUObj "(machine_word) option" word32 word32
+
+primrec
+  vcpuSCTLR :: "vcpu \<Rightarrow> word32"
+where
+  "vcpuSCTLR (VCPUObj v0 v1 v2) = v1"
+
+primrec
+  vcpuTCBPtr :: "vcpu \<Rightarrow> (machine_word) option"
+where
+  "vcpuTCBPtr (VCPUObj v0 v1 v2) = v0"
+
+primrec
+  vcpuACTLR :: "vcpu \<Rightarrow> word32"
+where
+  "vcpuACTLR (VCPUObj v0 v1 v2) = v2"
+
+primrec
+  vcpuSCTLR_update :: "(word32 \<Rightarrow> word32) \<Rightarrow> vcpu \<Rightarrow> vcpu"
+where
+  "vcpuSCTLR_update f (VCPUObj v0 v1 v2) = VCPUObj v0 (f v1) v2"
+
+primrec
+  vcpuTCBPtr_update :: "(((machine_word) option) \<Rightarrow> ((machine_word) option)) \<Rightarrow> vcpu \<Rightarrow> vcpu"
+where
+  "vcpuTCBPtr_update f (VCPUObj v0 v1 v2) = VCPUObj (f v0) v1 v2"
+
+primrec
+  vcpuACTLR_update :: "(word32 \<Rightarrow> word32) \<Rightarrow> vcpu \<Rightarrow> vcpu"
+where
+  "vcpuACTLR_update f (VCPUObj v0 v1 v2) = VCPUObj v0 v1 (f v2)"
+
+abbreviation (input)
+  VCPUObj_trans :: "((machine_word) option) \<Rightarrow> (word32) \<Rightarrow> (word32) \<Rightarrow> vcpu" ("VCPUObj'_ \<lparr> vcpuTCBPtr= _, vcpuSCTLR= _, vcpuACTLR= _ \<rparr>")
+where
+  "VCPUObj_ \<lparr> vcpuTCBPtr= v0, vcpuSCTLR= v1, vcpuACTLR= v2 \<rparr> == VCPUObj v0 v1 v2"
+
+lemma vcpuSCTLR_vcpuSCTLR_update [simp]:
+  "vcpuSCTLR (vcpuSCTLR_update f v) = f (vcpuSCTLR v)"
+  by (cases v) simp
+
+lemma vcpuSCTLR_vcpuTCBPtr_update [simp]:
+  "vcpuSCTLR (vcpuTCBPtr_update f v) = vcpuSCTLR v"
+  by (cases v) simp
+
+lemma vcpuSCTLR_vcpuACTLR_update [simp]:
+  "vcpuSCTLR (vcpuACTLR_update f v) = vcpuSCTLR v"
+  by (cases v) simp
+
+lemma vcpuTCBPtr_vcpuSCTLR_update [simp]:
+  "vcpuTCBPtr (vcpuSCTLR_update f v) = vcpuTCBPtr v"
+  by (cases v) simp
+
+lemma vcpuTCBPtr_vcpuTCBPtr_update [simp]:
+  "vcpuTCBPtr (vcpuTCBPtr_update f v) = f (vcpuTCBPtr v)"
+  by (cases v) simp
+
+lemma vcpuTCBPtr_vcpuACTLR_update [simp]:
+  "vcpuTCBPtr (vcpuACTLR_update f v) = vcpuTCBPtr v"
+  by (cases v) simp
+
+lemma vcpuACTLR_vcpuSCTLR_update [simp]:
+  "vcpuACTLR (vcpuSCTLR_update f v) = vcpuACTLR v"
+  by (cases v) simp
+
+lemma vcpuACTLR_vcpuTCBPtr_update [simp]:
+  "vcpuACTLR (vcpuTCBPtr_update f v) = vcpuACTLR v"
+  by (cases v) simp
+
+lemma vcpuACTLR_vcpuACTLR_update [simp]:
+  "vcpuACTLR (vcpuACTLR_update f v) = f (vcpuACTLR v)"
+  by (cases v) simp
 
 datatype arch_kernel_object =
     KOASIDPool asidpool
   | KOPTE pte
   | KOPDE pde
+  | KOVCPU vcpu
+
+datatype arch_tcb =
+    ArchThread user_context "(machine_word) option"
+
+primrec
+  atcbVCPUPtr :: "arch_tcb \<Rightarrow> (machine_word) option"
+where
+  "atcbVCPUPtr (ArchThread v0 v1) = v1"
+
+primrec
+  atcbContext :: "arch_tcb \<Rightarrow> user_context"
+where
+  "atcbContext (ArchThread v0 v1) = v0"
+
+primrec
+  atcbVCPUPtr_update :: "(((machine_word) option) \<Rightarrow> ((machine_word) option)) \<Rightarrow> arch_tcb \<Rightarrow> arch_tcb"
+where
+  "atcbVCPUPtr_update f (ArchThread v0 v1) = ArchThread v0 (f v1)"
+
+primrec
+  atcbContext_update :: "(user_context \<Rightarrow> user_context) \<Rightarrow> arch_tcb \<Rightarrow> arch_tcb"
+where
+  "atcbContext_update f (ArchThread v0 v1) = ArchThread (f v0) v1"
+
+abbreviation (input)
+  ArchThread_trans :: "(user_context) \<Rightarrow> ((machine_word) option) \<Rightarrow> arch_tcb" ("ArchThread'_ \<lparr> atcbContext= _, atcbVCPUPtr= _ \<rparr>")
+where
+  "ArchThread_ \<lparr> atcbContext= v0, atcbVCPUPtr= v1 \<rparr> == ArchThread v0 v1"
+
+lemma atcbVCPUPtr_atcbVCPUPtr_update [simp]:
+  "atcbVCPUPtr (atcbVCPUPtr_update f v) = f (atcbVCPUPtr v)"
+  by (cases v) simp
+
+lemma atcbVCPUPtr_atcbContext_update [simp]:
+  "atcbVCPUPtr (atcbContext_update f v) = atcbVCPUPtr v"
+  by (cases v) simp
+
+lemma atcbContext_atcbVCPUPtr_update [simp]:
+  "atcbContext (atcbVCPUPtr_update f v) = atcbContext v"
+  by (cases v) simp
+
+lemma atcbContext_atcbContext_update [simp]:
+  "atcbContext (atcbContext_update f v) = f (atcbContext v)"
+  by (cases v) simp
 
 consts'
 archObjSize :: "arch_kernel_object \<Rightarrow> nat"
@@ -211,15 +353,25 @@ asidRange :: "(asid * asid)"
 consts'
 asidHighBitsOf :: "asid \<Rightarrow> asid"
 
+consts'
+newVCPU :: "vcpu"
+
 defs archObjSize_def:
 "archObjSize a\<equiv> (case a of
-                  KOASIDPool v10 \<Rightarrow>   pageBits
-                | KOPTE v11 \<Rightarrow>   2
-                | KOPDE v12 \<Rightarrow>   2
+                  KOASIDPool v21 \<Rightarrow>   pageBits
+                | KOPTE v22 \<Rightarrow>   pteBits
+                | KOPDE v23 \<Rightarrow>   pdeBits
+                | KOVCPU v24 \<Rightarrow>   vcpuBits
                 )"
 
+definition
+"newArchTCB \<equiv> ArchThread_ \<lparr>
+    atcbContext= newContext
+    ,atcbVCPUPtr= Nothing
+    \<rparr>"
+
 defs asidHighBits_def:
-"asidHighBits \<equiv> 8"
+"asidHighBits \<equiv> 7"
 
 defs asidLowBits_def:
 "asidLowBits \<equiv> 10"
@@ -233,10 +385,14 @@ defs asidRange_def:
 defs asidHighBitsOf_def:
 "asidHighBitsOf asid\<equiv> (asid `~shiftR~` asidLowBits) && mask asidHighBits"
 
+defs newVCPU_def:
+"newVCPU \<equiv> error []"
+
 
 datatype arch_kernel_object_type =
     PDET
   | PTET
+  | VCPUT
   | ASIDPoolT
 
 primrec
@@ -244,7 +400,15 @@ primrec
 where
   "archTypeOf (KOPDE e) = PDET"
 | "archTypeOf (KOPTE e) = PTET"
+| "archTypeOf (KOVCPU e) = VCPUT"
 | "archTypeOf (KOASIDPool e) = ASIDPoolT"
+
+end
+
+context begin interpretation Arch .
+
+requalify_types
+  vcpu
 
 end
 end
