spec/design/ARM/ArchHypervisor_H.thy
@@ -1,0 +1,31 @@
+(*
+ * Copyright 2014, General Dynamics C4 Systems
+ *
+ * This software may be distributed and modified according to the terms of
+ * the GNU General Public License version 2. Note that NO WARRANTY is provided.
+ * See "LICENSE_GPLv2.txt" for details.
+ *
+ * @TAG(GD_GPL)
+ *)
+
+(* 
+  VSpace lookup code.
+*)
+
+theory ArchHypervisor_H
+imports
+  "../CNode_H"
+  "../KI_Decls_H"
+begin
+context Arch begin global_naming ARM_H
+
+
+consts'
+handleHypervisorFault :: "machine_word \<Rightarrow> hyp_fault_type \<Rightarrow> unit kernel"
+
+
+defs handleHypervisorFault_def:
+"handleHypervisorFault arg1 hyp \<equiv> case hyp of ARMNoHypFaults \<Rightarrow> haskell_fail []"
+
+end
+end
