spec/design/ARM_HYP/ArchFault_H.thy
@@ -1,0 +1,107 @@
+(*
+ * Copyright 2014, General Dynamics C4 Systems
+ *
+ * This software may be distributed and modified according to the terms of
+ * the GNU General Public License version 2. Note that NO WARRANTY is provided.
+ * See "LICENSE_GPLv2.txt" for details.
+ *
+ * @TAG(GD_GPL)
+ *)
+
+(* 
+  VSpace lookup code.
+*)
+
+theory ArchFault_H
+imports "../Types_H"
+(*  "../KI_Decls_H"
+  ArchVSpaceDecls_H *)
+begin
+context Arch begin global_naming ARM_HYP_H
+
+
+datatype arch_fault =
+    VMFault vptr "machine_word list"
+  | VCPUFault machine_word
+  | VGICMaintenance "machine_word list"
+
+primrec
+  vcpuHSR :: "arch_fault \<Rightarrow> machine_word"
+where
+  "vcpuHSR (VCPUFault v0) = v0"
+
+primrec
+  vmFaultAddress :: "arch_fault \<Rightarrow> vptr"
+where
+  "vmFaultAddress (VMFault v0 v1) = v0"
+
+primrec
+  vgicMaintenanceData :: "arch_fault \<Rightarrow> machine_word list"
+where
+  "vgicMaintenanceData (VGICMaintenance v0) = v0"
+
+primrec
+  vmFaultArchData :: "arch_fault \<Rightarrow> machine_word list"
+where
+  "vmFaultArchData (VMFault v0 v1) = v1"
+
+primrec
+  vcpuHSR_update :: "(machine_word \<Rightarrow> machine_word) \<Rightarrow> arch_fault \<Rightarrow> arch_fault"
+where
+  "vcpuHSR_update f (VCPUFault v0) = VCPUFault (f v0)"
+
+primrec
+  vmFaultAddress_update :: "(vptr \<Rightarrow> vptr) \<Rightarrow> arch_fault \<Rightarrow> arch_fault"
+where
+  "vmFaultAddress_update f (VMFault v0 v1) = VMFault (f v0) v1"
+
+primrec
+  vgicMaintenanceData_update :: "((machine_word list) \<Rightarrow> (machine_word list)) \<Rightarrow> arch_fault \<Rightarrow> arch_fault"
+where
+  "vgicMaintenanceData_update f (VGICMaintenance v0) = VGICMaintenance (f v0)"
+
+primrec
+  vmFaultArchData_update :: "((machine_word list) \<Rightarrow> (machine_word list)) \<Rightarrow> arch_fault \<Rightarrow> arch_fault"
+where
+  "vmFaultArchData_update f (VMFault v0 v1) = VMFault v0 (f v1)"
+
+abbreviation (input)
+  VMFault_trans :: "(vptr) \<Rightarrow> (machine_word list) \<Rightarrow> arch_fault" ("VMFault'_ \<lparr> vmFaultAddress= _, vmFaultArchData= _ \<rparr>")
+where
+  "VMFault_ \<lparr> vmFaultAddress= v0, vmFaultArchData= v1 \<rparr> == VMFault v0 v1"
+
+abbreviation (input)
+  VCPUFault_trans :: "(machine_word) \<Rightarrow> arch_fault" ("VCPUFault'_ \<lparr> vcpuHSR= _ \<rparr>")
+where
+  "VCPUFault_ \<lparr> vcpuHSR= v0 \<rparr> == VCPUFault v0"
+
+abbreviation (input)
+  VGICMaintenance_trans :: "(machine_word list) \<Rightarrow> arch_fault" ("VGICMaintenance'_ \<lparr> vgicMaintenanceData= _ \<rparr>")
+where
+  "VGICMaintenance_ \<lparr> vgicMaintenanceData= v0 \<rparr> == VGICMaintenance v0"
+
+definition
+  isVMFault :: "arch_fault \<Rightarrow> bool"
+where
+ "isVMFault v \<equiv> case v of
+    VMFault v0 v1 \<Rightarrow> True
+  | _ \<Rightarrow> False"
+
+definition
+  isVCPUFault :: "arch_fault \<Rightarrow> bool"
+where
+ "isVCPUFault v \<equiv> case v of
+    VCPUFault v0 \<Rightarrow> True
+  | _ \<Rightarrow> False"
+
+definition
+  isVGICMaintenance :: "arch_fault \<Rightarrow> bool"
+where
+ "isVGICMaintenance v \<equiv> case v of
+    VGICMaintenance v0 \<Rightarrow> True
+  | _ \<Rightarrow> False"
+
+
+
+end
+end
