spec/design/ARM_HYP/ArchInterrupt_H.thy
@@ -11,7 +11,7 @@
 theory ArchInterrupt_H
 imports "../RetypeDecls_H" "../CNode_H" "../InterruptDecls_H" ArchInterruptDecls_H
 begin
-context Arch begin global_naming ARM_H
+context Arch begin global_naming ARM_HYP_H
 
 defs decodeIRQControlInvocation_def:
 "decodeIRQControlInvocation arg1 arg2 arg3 arg4 \<equiv> throw IllegalOperation"
@@ -21,6 +21,15 @@ defs performIRQControl_def:
 
 defs checkIRQ_def:
 "checkIRQ irq\<equiv> rangeCheck irq (fromEnum minIRQ) (fromEnum maxIRQ)"
+
+defs handleReservedIRQ_def:
+"handleReservedIRQ irq \<equiv> haskell_fail []"
+
+defs initInterruptController_def:
+"initInterruptController\<equiv> (do
+    setIRQState IRQReserved $ IRQ irqVGICMaintenance;
+    return ()
+od)"
 
 
 end
