spec/design/ARM_HYP/ArchRetype_H.thy
@@ -17,26 +17,10 @@ imports
   Hardware_H
   "../KI_Decls_H"
 begin
-context Arch begin global_naming ARM_H
+context Arch begin global_naming ARM_HYP_H
 
 defs deriveCap_def:
-"deriveCap x0 x1\<equiv> (let c = x1 in
-  if isPageTableCap c \<and> capPTMappedAddress c \<noteq> None
-  then   returnOk c
-  else if isPageTableCap c \<and> capPTMappedAddress c = None
-  then   throw IllegalOperation
-  else if isPageDirectoryCap c \<and> capPDMappedASID c \<noteq> None
-  then   returnOk c
-  else if isPageDirectoryCap c \<and> capPDMappedASID c = None
-  then   throw IllegalOperation
-  else if isPageCap c
-  then   returnOk $ c \<lparr> capVPMappedAddress := Nothing \<rparr>
-  else if isASIDControlCap c
-  then   returnOk c
-  else if isASIDPoolCap c
-  then   returnOk c
-  else undefined
-  )"
+"deriveCap x0 x1\<equiv> (* case removed *) undefined"
 
 defs updateCapData_def:
 "updateCapData arg1 arg2 cap \<equiv> ArchObjectCap cap"
@@ -50,25 +34,7 @@ defs maskCapRights_def:
   )"
 
 defs finaliseCap_def:
-"finaliseCap x0 x1\<equiv> (case (x0, x1) of
-    ((ASIDPoolCap ptr b), True) \<Rightarrow>    (do
-    deleteASIDPool b ptr;
-    return NullCap
-    od)
-  | ((PageDirectoryCap ptr (Some a)), True) \<Rightarrow>    (do
-    deleteASID a ptr;
-    return NullCap
-  od)
-  | ((PageTableCap ptr (Some (a, v))), True) \<Rightarrow>    (do
-    unmapPageTable a v ptr;
-    return NullCap
-  od)
-  | ((PageCap ptr _ s (Some (a, v))), _) \<Rightarrow>    (do
-        unmapPage s a v ptr;
-        return NullCap
-  od)
-  | (_, _) \<Rightarrow>    return NullCap
-  )"
+"finaliseCap x0 x1\<equiv> (* case removed *) undefined"
 
 defs resetMemMapping_def:
 "resetMemMapping x0\<equiv> (case x0 of
@@ -79,79 +45,7 @@ defs resetMemMapping_def:
   )"
 
 defs recycleCap_def:
-"recycleCap is_final x1 \<equiv> (let cap = x1 in
-  if isPageCap cap
-  then   (do
-      doMachineOp $ clearMemory (capVPBasePtr cap)
-          (1 `~shiftL~` (pageBitsForSize $ capVPSize cap));
-      finaliseCap cap is_final;
-      return $ resetMemMapping cap
-  od)
-  else if isPageTableCap cap
-  then let ptr = capPTBasePtr cap
-  in   (do
-    pteBits \<leftarrow> return ( objBits InvalidPTE);
-    slots \<leftarrow> return ( [ptr, ptr + bit pteBits  .e.  ptr + bit ptBits - 1]);
-    mapM_x (flip storePTE InvalidPTE) slots;
-    doMachineOp $
-        cleanCacheRange_PoU (VPtr $ fromPPtr ptr)
-                            (VPtr $ fromPPtr ptr + (1 `~shiftL~` ptBits) - 1)
-                            (addrFromPPtr ptr);
-    (case capPTMappedAddress cap of
-          None \<Rightarrow>   return ()
-        | Some (a, v) \<Rightarrow>   (do
-            mapped \<leftarrow> pageTableMapped a v ptr;
-            when (mapped \<noteq> Nothing) $ invalidateTLBByASID a
-        od)
-        );
-    finaliseCap cap is_final;
-    return (if is_final then resetMemMapping cap else cap)
-  od)
-  else if isPageDirectoryCap cap
-  then let ptr = capPDBasePtr cap
-  in   (do
-    pdeBits \<leftarrow> return ( objBits InvalidPDE);
-    kBaseEntry \<leftarrow> return ( fromVPtr kernelBase
-                        `~shiftR~` pageBitsForSize ARMSection);
-    indices \<leftarrow> return ( [0  .e.  kBaseEntry - 1]);
-    offsets \<leftarrow> return ( map (PPtr \<circ> flip shiftL pdeBits) indices);
-    slots \<leftarrow> return ( map (\<lambda> x. x + ptr) offsets);
-    mapM_x (flip storePDE InvalidPDE) slots;
-    doMachineOp $
-        cleanCacheRange_PoU (VPtr $ fromPPtr ptr)
-                            (VPtr $ fromPPtr ptr + (1 `~shiftL~` pdBits) - 1)
-                            (addrFromPPtr ptr);
-    (case capPDMappedASID cap of
-          None \<Rightarrow>   return ()
-        | Some a \<Rightarrow>   (
-            ignoreFailure $ ((doE
-                pd' \<leftarrow> findPDForASID a;
-                withoutFailure $ when (ptr = pd') $ invalidateTLBByASID a
-            odE)
-                                                                          )
-        )
-        );
-    finaliseCap cap is_final;
-    return (if is_final then resetMemMapping cap else cap)
-  od)
-  else if isASIDControlCap cap
-  then   return ASIDControlCap
-  else if isASIDPoolCap cap
-  then let base = capASIDBase cap; ptr = capASIDPool cap
-  in   (do
-    asidTable \<leftarrow> gets (armKSASIDTable \<circ> ksArchState);
-    when (asidTable (asidHighBitsOf base) = Just ptr) $ (do
-        deleteASIDPool base ptr;
-        setObject ptr (makeObject ::asidpool);
-        asidTable \<leftarrow> gets (armKSASIDTable \<circ> ksArchState);
-        asidTable' \<leftarrow> return ( asidTable aLU [(asidHighBitsOf base, Just ptr)]);
-        modify (\<lambda> s. s \<lparr>
-            ksArchState := (ksArchState s) \<lparr> armKSASIDTable := asidTable' \<rparr>\<rparr>)
-    od);
-    return cap
-  od)
-  else undefined
-  )"
+"recycleCap is_final x1 \<equiv> (* case removed *) undefined"
 
 defs hasRecycleRights_def:
 "hasRecycleRights x0\<equiv> (case x0 of
@@ -160,30 +54,7 @@ defs hasRecycleRights_def:
   )"
 
 defs sameRegionAs_def:
-"sameRegionAs x0 x1\<equiv> (let (a, b) = (x0, x1) in
-  if isPageCap a \<and> isPageCap b
-  then 
-    let
-        botA = capVPBasePtr a;
-        botB = capVPBasePtr b;
-        topA = botA + bit (pageBitsForSize $ capVPSize a) - 1;
-        topB = botB + bit (pageBitsForSize $ capVPSize b) - 1
-    in
-    
-    (botA \<le> botB) \<and> (topA \<ge> topB) \<and> (botB \<le> topB)
-  else if isPageTableCap a \<and> isPageTableCap b
-  then  
-    capPTBasePtr a = capPTBasePtr b
-  else if isPageDirectoryCap a \<and> isPageDirectoryCap b
-  then  
-    capPDBasePtr a = capPDBasePtr b
-  else if isASIDControlCap a \<and> isASIDControlCap b
-  then   True
-  else if isASIDPoolCap a \<and> isASIDPoolCap b
-  then  
-    capASIDPool a = capASIDPool b
-  else   False
-  )"
+"sameRegionAs x0 x1\<equiv> (* case removed *) undefined"
 
 defs isPhysicalCap_def:
 "isPhysicalCap x0\<equiv> (case x0 of
@@ -211,70 +82,20 @@ od)"
 defs createObject_def:
 "createObject t regionBase arg3 \<equiv>
     let funupd = (\<lambda> f x v y. if y = x then v else f y) in
-    let pointerCast = PPtr \<circ> fromPPtr
-    in (case t of 
-        APIObjectType v2 \<Rightarrow> 
-            haskell_fail []
-        | SmallPageObject \<Rightarrow>  (do
-            createPageObject regionBase 0;
-            modify (\<lambda> ks. ks \<lparr> gsUserPages :=
-              funupd (gsUserPages ks)
-                     (fromPPtr regionBase) (Just ARMSmallPage)\<rparr>);
-            return $ PageCap (pointerCast regionBase)
-                  VMReadWrite ARMSmallPage Nothing
-        od)
-        | LargePageObject \<Rightarrow>  (do
-            createPageObject regionBase 4;
-            modify (\<lambda> ks. ks \<lparr> gsUserPages :=
-              funupd (gsUserPages ks)
-                     (fromPPtr regionBase) (Just ARMLargePage)\<rparr>);
-            return $ PageCap (pointerCast regionBase)
-                  VMReadWrite ARMLargePage Nothing
-        od)
-        | SectionObject \<Rightarrow>  (do
-            createPageObject regionBase 8;
-            modify (\<lambda> ks. ks \<lparr> gsUserPages :=
-              funupd (gsUserPages ks)
-                     (fromPPtr regionBase) (Just ARMSection)\<rparr>);
-            return $ PageCap (pointerCast regionBase)
-                  VMReadWrite ARMSection Nothing
-        od)
-        | SuperSectionObject \<Rightarrow>  (do
-            createPageObject regionBase 12;
-            modify (\<lambda> ks. ks \<lparr> gsUserPages :=
-              funupd (gsUserPages ks)
-                     (fromPPtr regionBase) (Just ARMSuperSection)\<rparr>);
-            return $ PageCap (pointerCast regionBase)
-                  VMReadWrite ARMSuperSection Nothing
-        od)
-        | PageTableObject \<Rightarrow>  (do
-            ptSize \<leftarrow> return ( ptBits - objBits (makeObject ::pte));
-            regionSize \<leftarrow> return ( (1 `~shiftL~` ptBits));
-            placeNewObject regionBase (makeObject ::pte) ptSize;
-            doMachineOp $
-                cleanCacheRange_PoU (VPtr $ fromPPtr regionBase)
-                      (VPtr $ fromPPtr regionBase + regionSize - 1)
-                      (addrFromPPtr regionBase);
-            return $ PageTableCap (pointerCast regionBase) Nothing
-        od)
-        | PageDirectoryObject \<Rightarrow>  (do
-            pdSize \<leftarrow> return ( pdBits - objBits (makeObject ::pde));
-            regionSize \<leftarrow> return ( (1 `~shiftL~` pdBits));
-            placeNewObject regionBase (makeObject ::pde) pdSize;
-            copyGlobalMappings (pointerCast regionBase);
-            doMachineOp $
-                cleanCacheRange_PoU (VPtr $ fromPPtr regionBase)
-                      (VPtr $ fromPPtr regionBase + regionSize - 1)
-                      (addrFromPPtr regionBase);
-            return $ PageDirectoryCap (pointerCast regionBase) Nothing
-        od)
-        )"
+    let pointerCast = PPtr \<circ> fromPPtr in
+    let mkPageCap = \<lambda> sz. PageCap (pointerCast regionBase) VMReadWrite sz Nothing
+    in (* case removed *) undefined"
 
 defs decodeInvocation_def:
-"decodeInvocation \<equiv> decodeARMMMUInvocation"
+"decodeInvocation label args capIndex slot cap extraCaps \<equiv>
+    (case cap of
+         VCPUCap _ \<Rightarrow>   decodeARMVCPUInvocation label args capIndex slot cap extraCaps
+       | _ \<Rightarrow>   decodeARMMMUInvocation label args capIndex slot cap extraCaps
+       )"
 
 defs performInvocation_def:
-"performInvocation \<equiv> performARMMMUInvocation"
+"performInvocation i \<equiv>
+    (* case removed *) undefined"
 
 defs capUntypedPtr_def:
 "capUntypedPtr x0\<equiv> (case x0 of
@@ -283,15 +104,17 @@ defs capUntypedPtr_def:
   | (PageDirectoryCap ((* PPtr *) p) _) \<Rightarrow>    PPtr p
   | ASIDControlCap \<Rightarrow>    error []
   | (ASIDPoolCap ((* PPtr *) p) _) \<Rightarrow>    PPtr p
+  | (VCPUCap ((* PPtr *) p)) \<Rightarrow>    PPtr p
   )"
 
 defs capUntypedSize_def:
 "capUntypedSize x0\<equiv> (case x0 of
-    (PageCap _ _ sz _) \<Rightarrow>    1 `~shiftL~` pageBitsForSize sz
-  | (PageTableCap _ _) \<Rightarrow>    1 `~shiftL~` 10
-  | (PageDirectoryCap _ _) \<Rightarrow>    1 `~shiftL~` 14
-  | (ASIDControlCap ) \<Rightarrow>    1 `~shiftL~` (asidHighBits + 2)
-  | (ASIDPoolCap _ _) \<Rightarrow>    1 `~shiftL~` (asidLowBits + 2)
+    (PageCap _ _ sz _) \<Rightarrow>    bit (pageBitsForSize sz)
+  | (PageTableCap _ _) \<Rightarrow>    bit (ptBits + pteBits)
+  | (PageDirectoryCap _ _) \<Rightarrow>    bit (pdBits + pdeBits)
+  | (ASIDControlCap ) \<Rightarrow>    bit (asidHighBits + 2)
+  | (ASIDPoolCap _ _) \<Rightarrow>    bit (asidLowBits + 2)
+  | (VCPUCap _) \<Rightarrow>    bit vcpuBits
   )"
 
 
