spec/design/ARM_HYP/Arch_Structs_B.thy
@@ -13,9 +13,9 @@
 chapter "Common, Architecture-Specific Data Types"
 
 theory Arch_Structs_B
-imports "~~/src/HOL/Main" "../../../spec/machine/Setup_Locale"
+imports "~~/src/HOL/Main" "../../machine/Setup_Locale"
 begin
-context Arch begin global_naming ARM_H
+context Arch begin global_naming ARM_HYP_H
 
 datatype arm_vspace_region_use =
     ArmVSpaceUserRegion
