spec/design/ARM_HYP/RegisterSet_H.thy
@@ -15,7 +15,7 @@ imports
   "../../../lib/HaskellLib_H"
   "../../machine/ARM_HYP/MachineTypes"
 begin
-context Arch begin global_naming ARM_H
+context Arch begin global_naming ARM_HYP_H
 
 definition
   newContext :: "register => machine_word"
